Upgrade version to 8.20 (#10)
* Add meta files from system-mp repository; update _CoqProject

* Delete old files and update import statements

* Update more import statements

* Remove tactics dependency for capturesets

* Update fsetdec to work with atoms and locs

* Add MetatheoryNat.v, adapted from old Nat.v

* Add nats and change var to original definition (temporary) in Metatheory.v

* Update names. Admitted a few proofs that no longer work.

* Update metatheory with store and new notation

* Update notation

* Update ccsub_definitions

* Add old "pick fresh" tactics to metatheory

* Update syntax of ccsub_infrastructure. Many admitted proofs that no longer work.

* Updated notation for ccsub_wellformedness. Many proofs left admitted.

* Comment out broken tactic

* Fix CaptureSets proofs

* Fix some proofs in ccsub_infra

* Update pick fresh notation to be different for locs

* Fix some proofs

* Update ccsub_lemmas, some proofs left admitted

* Update hints, subcapt, and subtyping. Some proofs
left admitted.

* Add atomset_subset_union lemma to Atom

* Update ccsub_typing, some proofs left admitted

* Fix pick fresh tactic in infrastructure

* Make everything up to substitution  build

---------

Co-authored-by: Samuel Li <sam674526@gmail.com>

CCsub_Definitions.v
@@ -1,11 +1,11 @@
-Require Export TaktikZ.
+(*Require Export TaktikZ.*)
 Require Export Metatheory.
 Require Export CaptureSets.
 Require Import Coq.Program.Wf.
 
-Notation "x '∈' L" := (x `in` L) (at level 80, no associativity).
-Notation "x '∉' L" := (x `notin` L) (at level 80, no associativity).
-Notation "xs '⊆' ys" := (xs `subset` ys) (at level 80, no associativity).
+Notation "x '∈' L" := (x `in`A L) (at level 80, no associativity).
+Notation "x '∉' L" := (x `notin`A L) (at level 80, no associativity).
+Notation "xs '⊆' ys" := (xs `subset`A ys) (at level 80, no associativity).
 
 Inductive typ : Type :=
   | typ_var : var -> typ
@@ -135,11 +135,11 @@ with pure_type : typ -> Prop :=
   | type_top : pure_type typ_top
   | type_arr : forall L S' T,
       type S' ->
-      (forall X : atom, X ∉ L -> type (open_ct T (cse_fvar X))) ->
+      (forall X : atom, X `notin`A L -> type (open_ct T (cse_fvar X))) ->
       pure_type (∀ (S') T)
   | type_all : forall L R T,
       pure_type R ->
-      (forall X : atom, X ∉ L -> type (open_tt T X)) ->
+      (forall X : atom, X `notin`A L -> type (open_tt T X)) ->
       pure_type (∀ [R] T)
   | type_box : forall T,
       type T ->
@@ -154,17 +154,17 @@ Inductive expr : exp -> Prop :=
       expr x
   | expr_abs : forall L T e1,
       type T ->
-      (forall x : atom, x ∉ L -> expr (open_ve e1 x (cse_fvar x))) ->
+      (forall x : atom, x `notin`A L -> expr (open_ve e1 x (cse_fvar x))) ->
       expr (λ (T) e1)
   | expr_app : forall (f x : var),
       expr (f @ x)
   | expr_let : forall L e1 e2,
       expr e1 ->
-      (forall x : atom, x ∉ L -> expr (open_ve e2 x (cse_fvar x))) ->
+      (forall x : atom, x `notin`A L -> expr (open_ve e2 x (cse_fvar x))) ->
       expr (let= e1 in e2)
   | expr_tabs : forall L R e1,
       pure_type R ->
-      (forall X : atom, X ∉ L -> expr (open_te e1 X)) ->
+      (forall X : atom, X `notin`A L -> expr (open_te e1 X)) ->
       expr (Λ [R] e1)
   | expr_tapp : forall (x : var) R,
       pure_type R ->
@@ -188,16 +188,16 @@ Notation "[ x ]" := (x :: nil).
 Definition allbound (Γ : ctx) (fvars : atoms) : Prop :=
   forall x,
     x `in`A fvars ->
-    exists C R, binds x (bind_typ (C # R)) Γ.
+    exists C R, EnvImpl.binds x (bind_typ (C # R)) Γ.
 
 Inductive wf_cse : ctx -> store_ctx -> cse -> Prop :=
   | wf_cse_top : forall Γ S,
       wf_cse Γ S cse_top
   | wf_cse_term_fvar : forall T S Γ (x : atom),
-      binds x (bind_typ T) Γ ->
+      EnvImpl.binds x (bind_typ T) Γ ->
       wf_cse Γ S (cse_fvar x)
   | wf_cse_term_loc : forall S T Γ (l : loc),
-      Store.binds l T S ->
+      binds l T S ->
       wf_cse Γ S (cse_loc l)
   | wf_cse_join : forall Γ S Q1 Q2,
       wf_cse Γ S Q1 ->
@@ -208,18 +208,18 @@ Inductive wf_cse : ctx -> store_ctx -> cse -> Prop :=
 
 Inductive wf_typ : ctx -> store_ctx -> typ -> Prop :=
   | wf_typ_var : forall Γ S X T,
-      binds X (bind_sub T) Γ ->
+      EnvImpl.binds X (bind_sub T) Γ ->
       wf_typ Γ S X
   | wf_typ_top : forall Γ S,
       wf_typ Γ S typ_top
   | wf_typ_arr : forall L Γ S C R T,
       wf_typ Γ S (C # R) ->
-      (forall x : atom, x ∉ L -> wf_typ ([(x, bind_typ (C # R))] ++ Γ) S (open_ct T (cse_fvar x))) ->
+      (forall x : atom, x `notin`A L -> wf_typ ([(x, bind_typ (C # R))] ++ Γ) S (open_ct T (cse_fvar x))) ->
       wf_typ Γ S (∀ (C # R) T)
   | wf_typ_all : forall L S Γ R T,
       wf_typ Γ S R ->
       pure_type R ->
-      (forall X : atom, X ∉ L -> wf_typ ([(X, bind_sub R)] ++ Γ) S (open_tt T X)) ->
+      (forall X : atom, X `notin`A L -> wf_typ ([(X, bind_sub R)] ++ Γ) S (open_tt T X)) ->
       wf_typ Γ S (∀ [R] T)
   | wf_typ_box : forall Γ S T,
       wf_typ Γ S T ->
@@ -232,7 +232,7 @@ Inductive wf_typ : ctx -> store_ctx -> typ -> Prop :=
 
 Reserved Notation "S '∷' Γ" (at level 40, Γ at next level, no associativity).
 Reserved Notation "Γ '⊢' E ':' S '⇒' T" (at level 40, E at next level, S at next level, T at next level, no associativity).
-Reserved Notation "Σ1 '-->' Σ2" (at level 40, Σ2 at next level, no associativity).
+Reserved Notation "Σ1 '--->' Σ2" (at level 40, Σ2 at next level, no associativity).
 
 Inductive wf_store_ctx : store_ctx -> Prop :=
   | wf_store_ctx_nil :
@@ -240,7 +240,7 @@ Inductive wf_store_ctx : store_ctx -> Prop :=
   | wf_store_ctx_cons : forall l S C R,
       wf_store_ctx S ->
       wf_typ nil S (C # R) ->
-      l `Notin` (Store.dom S) ->
+      l `notin`L (StoreImpl.dom S) ->
       wf_store_ctx ([(l, C # R)] ++ S).
 
 Inductive wf_ctx : ctx -> store_ctx -> Prop :=
@@ -251,12 +251,12 @@ Inductive wf_ctx : ctx -> store_ctx -> Prop :=
       wf_ctx Γ S ->
       wf_typ Γ S T ->
       pure_type T ->
-      X ∉ dom Γ ->
+      X ∉ EnvImpl.dom Γ ->
       wf_ctx ([(X, bind_sub T)] ++ Γ) S
   | wf_ctx_typ : forall (Γ : ctx) (S : store_ctx) (x : atom) (C : cse) (R : typ),
       wf_ctx Γ S ->
       wf_typ Γ S (C # R) ->
-      x ∉ dom Γ ->
+      x ∉ EnvImpl.dom Γ ->
       wf_ctx ([(x, bind_typ (C # R))] ++ Γ) S.
 
 Inductive subcapt : ctx -> store_ctx -> cse -> cse -> Prop :=
@@ -277,11 +277,11 @@ Inductive subcapt : ctx -> store_ctx -> cse -> cse -> Prop :=
       wf_cse Γ S (cse_loc l) ->
       subcapt Γ S (cse_loc l) (cse_loc l)
   | subcapt_trans_var : forall R S Γ Q X T,
-      binds X (bind_typ (typ_capt R T)) Γ ->
+      EnvImpl.binds X (bind_typ (typ_capt R T)) Γ ->
       subcapt Γ S R Q ->
       subcapt Γ S (cse_fvar X) Q
   | subcapt_trans_loc : forall Γ R S Q l T,
-      Store.binds l (typ_capt R T) S ->
+      binds l (typ_capt R T) S ->
       subcapt Γ S R Q ->
       subcapt Γ S (cse_loc l) Q
   | subcapt_join_inl : forall Γ S R1 R2 Q,
@@ -303,7 +303,7 @@ Inductive sub : ctx -> store_ctx -> typ -> typ -> Prop :=
       wf_typ Γ S X ->
       sub Γ S X X
   | sub_trans_tvar : forall U S Γ T X,
-      binds X (bind_sub U) Γ ->
+      EnvImpl.binds X (bind_sub U) Γ ->
       sub Γ S U T ->
       sub Γ S X T
   | sub_capt : forall Γ S C1 C2 R1 R2,
@@ -337,7 +337,7 @@ Inductive sub : ctx -> store_ctx -> typ -> typ -> Prop :=
 Inductive typing : ctx -> store_ctx -> exp -> typ -> Prop :=
   | typing_var : forall Γ x S C R,
       wf_ctx Γ S ->
-      binds x (bind_typ (C # R)) Γ ->
+      EnvImpl.binds x (bind_typ (C # R)) Γ ->
       typing Γ S x (cse_fvar x # R)
   | typing_abs : forall L Γ C R e1 T1 S,
       wf_typ Γ S (C # R) ->
