CCsub_Inversion.v
@@ -1,3 +1,4 @@
+Require Import TaktikZ.
 Require Import Coq.Program.Equality.
 Require Import LibTactics.
 Require Export CCsub_Hints.
@@ -7,6 +8,7 @@ Require Import CCsub_Typing.
 
 (* ********************************************************************** *)
 (** ** Inversion of typing (13) *)
+
 
 Lemma typing_inv_abs : forall Γ S1 e1 T S,
   typing Γ S (λ (S1) e1) T ->
@@ -19,21 +21,19 @@ Lemma typing_inv_abs : forall Γ S1 e1 T S,
 Proof with auto.
   intros * Typ.
   dependent induction Typ; intros U1 U2 D Sub.
-  - Case "typing_abs".
-    inversion Sub; subst.
+  - inversion Sub; subst.
     inversion select (sub _ _ _ _); subst.
     split...
     exists T1.
-    exists (L `u`A L0).
+    exists (L `union`A L0).
     intros y ?.
     rename select (forall x : atom, x ∉ L0 -> _) into Sub'.
     specialize (Sub' y ltac:(fsetdec)).
     repeat split...
-    rewrite_nil_concat.
+    rewrite_env (nil ++ [(y, bind_typ (C # R))] ++ Γ).
     eapply wf_typ_ignores_typ_bindings.
     applys sub_regular Sub'.
-  - Case "typing_sub".
-    eauto using (sub_transitivity T).
+  - eauto using (sub_transitivity T).
 Qed.
 
 Lemma typing_inv_tabs : forall Γ S1 e1 T S,
@@ -43,21 +43,19 @@ Lemma typing_inv_tabs : forall Γ S1 e1 T S,
   /\ exists S2, exists L, forall X, X ∉ L ->
     typing ([(X, bind_sub U1)] ++ Γ) S (open_te e1 X) (open_tt S2 X) /\
     sub ([(X, bind_sub U1)] ++ Γ) S (open_tt S2 X) (open_tt U2 X).
-Proof with simpl_env; auto.
+Proof with simpl_env; eauto.
   intros * Typ.
   dependent induction Typ; intros U1 U2 D Sub.
-  - Case "typing_tabs".
-    inversion Sub; subst.
+  - inversion Sub; subst.
     inversion select (sub _ _ _ _); subst.
     split...
     exists T1.
-    exists (L `union` L0).
+    exists (L `union`A L0).
     intros Y ?.
     repeat split...
-    rewrite_nil_concat.
+    rewrite_env (nil ++ [(Y, bind_sub U1)] ++ Γ).
     eapply typing_narrowing with (Q := S1)...
-  - Case "typing_sub".
-    eauto using (sub_transitivity T).
+  - eauto using (sub_transitivity T).
 Qed.
 
 Lemma typing_inv_let : forall Γ e k T S,
@@ -66,13 +64,13 @@ Lemma typing_inv_let : forall Γ e k T S,
     typing Γ S e (C # R)
     /\ exists L, forall x, x ∉ L ->
       typing ([(x, bind_typ (C # R))] ++ Γ) S (open_ve k x (cse_fvar x)) T.
-Proof with eauto*.
+Proof with eauto.
   intros * Typ.
   dependent induction Typ...
   destruct (IHTyp e k ltac:(reflexivity)) as [C [R0 [eTyp [L kTyp]]]].
   exists C, R0.
   split...
-  exists (L `u`A dom Γ).
+  exists (L `union`A EnvImpl.dom Γ).
   intros y NotIn.
   specialize (kTyp y ltac:(clear - NotIn; fsetdec)).
   apply typing_sub with (R := R)...
@@ -85,15 +83,13 @@ Lemma typing_inv_app : forall Γ S (f x : atom) T,
   exists C D Q U, typing Γ S f (C # (∀ (D # Q) U))
                /\ typing Γ S x (D # Q)
                /\ sub Γ S (open_ct U (cse_fvar x)) T.
-Proof with eauto*.
+Proof with eauto.
   intros * Typ.
   forwards (WfStore & WfCtx & _ & WfT): typing_regular Typ.
   dependent induction Typ.
-  - Case "typing_app".
-    repeat eexists...
+  - repeat eexists...
     apply sub_reflexivity...
-  - Case "typing_sub".
-    rename select (sub Γ S R T) into Sub.
+  - rename select (sub Γ S R T) into Sub.
     assert (WfR : wf_typ Γ S R) by applys sub_regular Sub.
     destruct (IHTyp f x ltac:(reflexivity) WfStore WfCtx WfR) as [C [D [Q [U [fTyp [xTyp Sub']]]]]].
     repeat eexists...
@@ -105,11 +101,10 @@ Lemma typing_inv_tapp : forall Γ S (x : atom) V T,
   exists C R U, typing Γ S x (C # (∀ [R] U))
              /\ sub Γ S V R
              /\ sub Γ S (open_tt U V) T.
-Proof with eauto*.
+Proof with eauto.
   intros * Typ.
   dependent induction Typ.
-  - Case "typing_tapp".
-    exists C, Q, T.
+  - exists C, Q, T.
     repeat split...
     apply sub_reflexivity...
     forwards (WfStore & WCtx & _ & WfCQT): typing_regular Typ.
@@ -117,13 +112,9 @@ Proof with eauto*.
     inversion select (wf_typ Γ S (∀ [Q] T)); subst.
     rename select (forall X : atom, X ∉ L -> wf_typ _ _ _) into WfT.
     pick fresh Y and specialize WfT.
-    replace (open_tt T V) with (subst_tt Y V (open_tt T Y)) by (rewrite <- subst_tt_intro; eauto).
-    rewrite_env (map (subst_tb Y V) nil ++ Γ).
-    eapply wf_typ_subst_tb...
-    + applys sub_pure_type...
-    + apply ok_cons...
-  - Case "typing_sub".
-    destruct (IHTyp x V eq_refl) as [C [R' [U [fTyp [lTyp Sub]]]]].
+    eapply wf_typ_open_type...
+    epose proof ((proj2 (sub_pure_type _ _ _ _ H)) H8)...
+  - destruct (IHTyp x V eq_refl) as [C [R' [U [fTyp [lTyp Sub]]]]].
     exists C, R', U.
     repeat split...
     apply sub_transitivity with (Q := R)...
@@ -132,22 +123,20 @@ Qed.
 Lemma typing_inv_box : forall Γ S x T,
   typing Γ S (box x) T ->
   exists C R, typing Γ S x (C # R)
-           /\ `cse_fvars` C ⊆ dom Γ
+           /\ `cse_fvars` C ⊆ EnvImpl.dom Γ
            /\ sub Γ S ({} # □ (C # R)) T.
-Proof with eauto*.
+Proof with eauto.
   intros * Typ.
   forwards (WfStore & WfCtx & _ & WfT): typing_regular Typ.
   dependent induction Typ...
-  - Case "typing_box".
-    exists C, R.
+  - exists C, R.
     repeat split...
     + intros x InC.
       apply wf_cse_free_vars_bound with (X := x) in H...
       destruct H as [T Binds].
-      apply binds_In with (a := bind_typ T)...
+      apply EnvImpl.binds_In with (a := bind_typ T)...
     + apply sub_reflexivity...
-  - Case "typing_sub".
-    rename select (sub Γ S R T) into Sub.
+  - rename select (sub Γ S R T) into Sub.
     assert (WfR : wf_typ Γ S R) by applys sub_regular Sub.
     destruct (IHTyp x eq_refl WfStore WfCtx WfR) as [C [R' [lTyp [xSubΓ CRsubS]]]].
     exists C, R'.
@@ -159,16 +148,14 @@ Lemma typing_inv_unbox : forall Γ S C x T,
   typing Γ S (exp_unbox C x) T ->
   exists R, typing Γ S x ({} # (□ (C # R)))
          /\ sub Γ S (C # R) T.
-Proof with eauto*.
+Proof with eauto.
   intros * Typ.
   forwards (WfStore & WfCtx & _ & WfT): typing_regular Typ.
   dependent induction Typ...
-  - Case "typing_unbox".
-    exists R.
+  - exists R.
     repeat split...
     apply sub_reflexivity...
-  - Case "typing_sub".
-    rename select (sub Γ S R T) into Sub.
+  - rename select (sub Γ S R T) into Sub.
     assert (WfR : wf_typ Γ S R) by applys sub_regular Sub.
     destruct (IHTyp _ _ eq_refl WfStore WfCtx WfR) as [R' [xTyp CRsubS]].
     exists R'.
