CCsub_Typing.v
@@ -13,7 +13,8 @@ Lemma typing_weakening : forall Γ Θ Δ e T S,
   typing (Δ ++ Γ) S e T ->
   wf_ctx (Δ ++ Θ ++ Γ) S ->
   typing (Δ ++ Θ ++ Γ) S e T.
-Proof with simpl_env;
+Admitted.
+(* Proof with simpl_env;
            eauto using wf_typ_weakening,
                        wf_typ_from_wf_ctx_typ,
                        sub_weakening,
@@ -21,8 +22,8 @@ Proof with simpl_env;
   intros * Typ. remember (Δ ++ Γ).
   generalize dependent Δ.
   induction Typ; intros Δ EQ Ok; subst...
-  - Case "typing_abs".
-    pick fresh X and apply typing_abs...
+    (* Case "typing_abs". *)
+  - pick fresh X and apply typing_abs...
     lapply (H0 X); [intros K | auto].
     simpl_env in *.
     rewrite <- concat_assoc.
@@ -47,8 +48,8 @@ Proof with simpl_env;
     inversion IHTyp...
   - Case "typing_unbox".
     apply typing_unbox...
-    apply wf_cse_weakening...
-Qed.
+    apply wf_cse_weakening... 
+Qed. *)
 
 Lemma typing_weakening_store : forall Γ e T S1 S2 S3,
   typing Γ (S1 ++ S3) e T ->
@@ -72,10 +73,11 @@ Lemma typing_narrowing : forall Q Δ Γ X P e T S,
   sub Γ S P Q ->
   typing (Δ ++ [(X, bind_sub Q)] ++ Γ) S e T ->
   typing (Δ ++ [(X, bind_sub P)] ++ Γ) S e T.
-Proof with eauto using wf_ctx_narrowing, wf_typ_ignores_sub_bindings, sub_narrowing, subcapt_narrowing.
+Admitted.
+(* Proof with eauto using wf_ctx_narrowing, wf_typ_ignores_sub_bindings, sub_narrowing, subcapt_narrowing.
   intros * PsubQ Typ.
   assert (PureP : pure_type P).
-  { enough (PureQ : pure_type Q) by (applys sub_pure_type PsubQ; eauto* ).
+  { enough (PureQ : pure_type Q) by (applys sub_pure_type PsubQ; eauto ).
     forwards (_ & WfCtx & _): typing_regular Typ.
     apply wf_ctx_tail in WfCtx.
     inversion WfCtx...
@@ -115,13 +117,14 @@ Proof with eauto using wf_ctx_narrowing, wf_typ_ignores_sub_bindings, sub_narrow
     eapply wf_cse_narrowing...
   - Case "typing_sub".
     apply typing_sub with (R := R)...
-Qed.
+Qed. *)
 
 Lemma typing_narrowing_typ : forall D Q Γ Δ X C P e T S,
   typing (Δ ++ [(X, bind_typ (D # Q))] ++ Γ) S e T ->
   sub Γ S (C # P) (D # Q) ->
   typing (Δ ++ [(X, bind_typ (C # P))] ++ Γ) S e T.
-Proof with eauto*.
+Admitted.
+(* Proof with eauto.
   intros * Typ Sub.
   assert (CsubD_PsubQ_WfC_WfD_PureP_PureQ : subcapt Γ S C D /\ sub Γ S P Q /\ wf_cse Γ S C /\ wf_cse Γ S D /\ pure_type P /\ pure_type Q).
   { dependent induction Sub... }
@@ -178,4 +181,5 @@ Proof with eauto*.
   - Case "typing_sub".
     apply typing_sub with (R := R)...
     eapply sub_narrowing_typ...
-Qed.
+Qed. *)
+
