Meta/MetatheoryNat.v
@@ -1,0 +1,63 @@
+Require Import Coq.Arith.Arith.
+Require Import Coq.Classes.EquivDec.
+Require Import Coq.Lists.List.
+Require Import Coq.Structures.Equalities.
+
+Require Import Coq.FSets.FSets.
+Require Import CoqListFacts.
+Require Import FSetExtra.
+Require Import FSetWeakNotin.
+Require Import LibTactics.
+
+Require Import List.
+(* Require Import Max. *)
+Require Import OrderedTypeEx.
+Require Import OrderedType.
+
+Require Import FSetDecide.
+Require Import FSetFacts.
+
+(** Helpers, defining a set of natural numbers. *)
+Module Type NATSET <: UsualDecidableType.
+    Definition t := nat.
+    (* Declare Module OT : UsualOrderedType with Definition t := nat. *)
+    Parameter eq_dec : forall x y : nat, {x = y} + {x <> y}.
+
+    #[global]
+    Hint Resolve eq_dec : core.
+
+    Include HasUsualEq <+ UsualIsEq <+ UsualIsEqOrig.
+End NATSET.
+
+(** The implementation of the above interface is hidden for
+    documentation purposes. *)
+
+Module NatSet : NATSET.
+    (* begin hide *)
+    Definition t := nat.
+    Module OT := Nat_as_OT.
+    Module Facts := OrderedTypeFacts OT.
+    Definition eq_dec : forall x y : nat, {x = y} + {x <> y} := 
+        Facts.eq_dec. 
+
+    Include HasUsualEq <+ UsualIsEq <+ UsualIsEqOrig.
+  (* end hide *)
+End NatSet.
+
+(** Defining a set of Natural Numbers. *)
+Module NatSetImpl : FSetExtra.WSfun NatSet :=
+  FSetExtra.Make NatSet.
+
+(** The type [nats] is the type of finite sets of [nat]s. *)
+Notation nats := NatSetImpl.t.
+Notation "{}N" :=
+  NatSetImpl.empty : metatheory_scope.
+
+(** We instantiate two modules which provide useful lemmas and tactics
+    work working with finite sets of atoms. *)
+
+Module NatSetDecide := Coq.FSets.FSetDecide.WDecide_fun NatSet NatSetImpl.
+Module NatSetNotin  := FSetWeakNotin.Notin_fun   NatSet NatSetImpl.
+Module NatSetFacts  := FSetFacts.WFacts_fun NatSet NatSetImpl.
+Module NatSetProperties := FSetProperties.WProperties_fun NatSet NatSetImpl.
+
